feat(proof-libs/fstar): add `lemma_get_bit_bounded`

proof-libs/fstar/rust_primitives/Rust_primitives.BitVectors.fst
@@ -8,6 +8,8 @@ open Rust_primitives.Integers
 
 let lemma_get_bit_bounded #t x d i = admit()
 
+let lemma_get_bit_bounded' #t x d = admit()
+
 let pow2_minus_one_mod_lemma1 (n: nat) (m: nat {m < n})
    : Lemma (((pow2 n - 1) / pow2 m) % 2 == 1)
    = let d: pos = n - m in
